elaborated basic

Games/gameLib/Basic.lean
@@ -6,25 +6,12 @@ Author: Yves Jäckle.
 
 
 import Mathlib.Tactic
+import Games.exLib.Nat
 
 
+-- # Environments
 
-/--
-### Games
 
-Games are determined 2 types:
-- `α`, the type representing the state of the game
-- `β`, the type representing actions
-
-As well as 4 data:
-
-- `init_game_state` : the intitial state of the game
-- `transition` : a function taking the current state and current action as input
-                 and returning the next state as output. The uniqueness of this
-                 transition function assumes that transitions are independent of
-                 which player has the turn.
--
--/
 structure Game_World (α β : Type u) where
   /-- Inital state-/
   init_game_state : α
@@ -54,30 +41,123 @@ structure Symm_Game_World (α β : Type u) where
   law : List β → (β → Prop)
 
 
+def Symm_Game_World.toGame_World {α β : Type u} (g : Symm_Game_World α β) : Game_World α β :=
+  {init_game_state := g.init_game_state
+   fst_win_states := g.win_states
+   fst_transition := g.transition
+   fst_legal := g.law
+   snd_win_states := g.win_states
+   snd_transition := g.transition
+   snd_legal := g.law
+   }
+
+
+instance {α β : Type u} : Coe (Symm_Game_World α β) (Game_World α β) where
+  coe := Symm_Game_World.toGame_World
+
+@[simp]
+lemma Symm_Game_World.toGame_World_ini {α β : Type u} (g : Symm_Game_World α β) :
+  g.toGame_World.init_game_state = g.init_game_state :=
+  by
+  rfl
+
+@[simp]
+lemma Symm_Game_World.toGame_World_fst_win {α β : Type u} (g : Symm_Game_World α β) :
+  g.toGame_World.fst_win_states = g.win_states :=
+  by
+  rfl
+
+@[simp]
+lemma Symm_Game_World.toGame_World_snd_win {α β : Type u} (g : Symm_Game_World α β) :
+  g.toGame_World.snd_win_states = g.win_states :=
+  by
+  rfl
+
+@[simp]
+lemma Symm_Game_World.toGame_World_fst_trans {α β : Type u} (g : Symm_Game_World α β) :
+  g.toGame_World.fst_transition = g.transition :=
+  by
+  rfl
+
+@[simp]
+lemma Symm_Game_World.toGame_World_snd_trans {α β : Type u} (g : Symm_Game_World α β) :
+  g.toGame_World.snd_transition = g.transition :=
+  by
+  rfl
+
+@[simp]
+lemma Symm_Game_World.toGame_World_fst_legal {α β : Type u} (g : Symm_Game_World α β) :
+  g.toGame_World.fst_legal = g.law :=
+  by
+  rfl
+
+@[simp]
+lemma Symm_Game_World.toGame_World_snd_legal {α β : Type u} (g : Symm_Game_World α β) :
+  g.toGame_World.snd_legal = g.law :=
+  by
+  rfl
+
 /--
 The list of actions represents the history of actions taken
 by both players. From the history and initial state (first input),
 one may deduce the current state, which may be used to define
 startegies.
 -/
-abbrev Game.strategy (α β : Type u) := α → List β → β
+abbrev Strategy (α β : Type u) := α → List β → β
 
-abbrev Game.strategy_legal {α β : Type u}
-  (ini : α) (law : List β → (β → Prop)) (strat : Game.strategy α β): Prop :=
-  ∀ hist : List β, law hist (strat ini hist)
+def Strategy_legal_at {α β : Type u}
+  (ini : α) (hist : List β) (law : α → List β → (β → Prop)) (strat : Strategy α β): Prop :=
+  law ini hist (strat ini hist)
+
+
+/-- Turn 0 represents initial state, then turns represent the state after the action-/
+def Turn_fst (turn : ℕ): Prop := turn % 2 = 1
+
+def Turn_snd (turn : ℕ): Prop := ¬ (turn % 2 = 1)
+
+instance : DecidablePred Turn_fst :=
+  fun turn => by rw [Turn_fst] ; exact Nat.decEq (turn % 2) 1
+
+instance : DecidablePred Turn_snd :=
+  fun turn => by rw [Turn_snd] ; exact Not.decidable
+
+abbrev Turn_from_hist {β : Type u} (hist : List β) := hist.length + 1
+
+
+def History_on_turn {α β : Type u}
+    (ini : α) (fst_strat snd_strat: Strategy α β) : ℕ → List β
+| 0 => []
+| n+1 => let h := History_on_turn ini fst_strat snd_strat n
+         if Turn_fst (n+1)
+         then (fst_strat ini h) :: h
+         else (snd_strat ini h) :: h
+
+
+abbrev Strategy_legal {α β : Type u}
+  (ini : α) (law : α → List β → (β → Prop)) (f_strat s_strat strat : Strategy α β): Prop :=
+  ∀ turn : ℕ, law ini (History_on_turn ini f_strat s_strat turn) (strat ini (History_on_turn ini f_strat s_strat turn))
 
 structure Game (α β : Type u) extends Game_World α β where
-  fst_strat : Game.strategy α β
-  fst_lawful :  Game.strategy_legal init_game_state fst_legal fst_strat
-  snd_strat : Game.strategy α β
-  snd_lawful : Game.strategy_legal init_game_state snd_legal snd_strat
+  fst_strat : Strategy α β
+  snd_strat : Strategy α β
+  fst_lawful : Strategy_legal init_game_state (fun _ => fst_legal) fst_strat snd_strat fst_strat
+  snd_lawful : Strategy_legal init_game_state (fun _ => snd_legal) fst_strat snd_strat snd_strat
 
 
 structure Symm_Game (α β : Type u) extends Symm_Game_World α β where
-  fst_strat : Game.strategy α β
-  fst_lawful :  Game.strategy_legal init_game_state law fst_strat
-  snd_strat : Game.strategy α β
-  snd_lawful : Game.strategy_legal init_game_state law snd_strat
+  fst_strat : Strategy α β
+  snd_strat : Strategy α β
+  fst_lawful : ∀ turn : ℕ, Strategy_legal_at
+                            init_game_state
+                            (History_on_turn init_game_state fst_strat snd_strat turn)
+                            (fun _ => law)
+                            fst_strat
+  snd_lawful : ∀ turn : ℕ, Strategy_legal_at
+                            init_game_state
+                            (History_on_turn init_game_state fst_strat snd_strat turn)
+                            (fun _ => law)
+                            snd_strat
+
 
 def Symm_Game.toGame {α β : Type u} (g : Symm_Game α β) : Game α β :=
  {init_game_state := g.init_game_state
@@ -94,180 +174,576 @@ def Symm_Game.toGame {α β : Type u} (g : Symm_Game α β) : Game α β :=
   }
 
 
--- structure Symm_Game (α β : Type u) extends Game α β where
---   win_symm : fst_win_states = snd_win_states
---   transition_symm : fst_transition = snd_transition
---   legal_symm : fst_legal = snd_legal
+@[simp]
+lemma Symm_Game.toGame_ini {α β : Type u} (g : Symm_Game α β) :
+  g.toGame.init_game_state = g.init_game_state :=
+  by
+  rfl
+
+@[simp]
+lemma Symm_Game.toGame_fst_win {α β : Type u} (g : Symm_Game α β) :
+  g.toGame.fst_win_states = g.win_states :=
+  by
+  rfl
+
+@[simp]
+lemma Symm_Game.toGame_snd_win {α β : Type u} (g : Symm_Game α β) :
+  g.toGame.snd_win_states = g.win_states :=
+  by
+  rfl
+
+@[simp]
+lemma Symm_Game.toGame_fst_trans {α β : Type u} (g : Symm_Game α β) :
+  g.toGame.fst_transition = g.transition :=
+  by
+  rfl
+
+@[simp]
+lemma Symm_Game.toGame_snd_trans {α β : Type u} (g : Symm_Game α β) :
+  g.toGame.snd_transition = g.transition :=
+  by
+  rfl
+
+@[simp]
+lemma Symm_Game.toGame_fst_legal {α β : Type u} (g : Symm_Game α β) :
+  g.toGame.fst_legal = g.law :=
+  by
+  rfl
+
+@[simp]
+lemma Symm_Game.toGame_snd_legal {α β : Type u} (g : Symm_Game α β) :
+  g.toGame.snd_legal = g.law :=
+  by
+  rfl
+
+@[simp]
+lemma Symm_Game.toGame_fst_strat {α β : Type u} (g : Symm_Game α β) :
+  g.toGame.fst_strat = g.fst_strat :=
+  by
+  rfl
+
+@[simp]
+lemma Symm_Game.toGame_snd_start {α β : Type u} (g : Symm_Game α β) :
+  g.toGame.snd_strat = g.snd_strat :=
+  by
+  rfl
+
+instance {α β : Type u} : Coe (Symm_Game α β) (Game α β) where
+  coe := Symm_Game.toGame
+
+@[simp]
+lemma Symm_Game.toGame_toWorld {α β : Type u} (g : Symm_Game α β):
+  g.toGame.toGame_World = g.toSymm_Game_World.toGame_World :=
+  by
+  dsimp [Symm_Game.toGame, Game.toGame_World, Symm_Game.toSymm_Game_World, Symm_Game_World.toGame_World]
 
 
--- def Symm_Game.build {α β : Type u}
---  (init : α)
---  (win_states : α → Prop)
---  (transition : List β → β → α)
---  (law : List β → (β → Prop))
---  (f_strat s_strat: Game.strategy α β)
---  (f_lawful :  Game.strategy_legal init law f_strat)
---  (s_lawful :  Game.strategy_legal init law s_strat) :
---  Symm_Game α β where
---   init_game_state := init
---   fst_win_states := win_states
---   fst_transition := transition
---   snd_win_states := win_states
---   snd_transition := transition
---   fst_strat := f_strat
---   snd_strat := s_strat
---   fst_legal := law
---   snd_legal := law
---   fst_lawful := f_lawful
---   snd_lawful := s_lawful
---   win_symm := by rfl
---   transition_symm := by rfl
---   legal_symm := by rfl
-
--- def Symm_Game.from_world {α β : Type u} (g : Symm_Game_World α β)
---  (f_strat s_strat: Game.strategy α β)
---  (f_lawful :  Game.strategy_legal g.init_game_state g.law f_strat)
---  (s_lawful :  Game.strategy_legal  g.init_game_state g.law s_strat) :
---  Symm_Game α β where
---   init_game_state := g.init_game_state
---   fst_win_states := g.win_states
---   fst_transition := g.transition
---   snd_win_states := g.win_states
---   snd_transition := g.transition
---   fst_strat := f_strat
---   snd_strat := s_strat
---   fst_legal := g.law
---   snd_legal := g.law
---   fst_lawful := f_lawful
---   snd_lawful := s_lawful
---   win_symm := by rfl
---   transition_symm := by rfl
---   legal_symm := by rfl
-
-
-/-- Turn 0 represents initial state, then turns represent the state after the action-/
-def Game.turn_fst (turn : ℕ): Prop := turn % 2 = 1
-
-def Game.turn_snd (turn : ℕ): Prop := ¬ (turn % 2 = 1)
-
-instance : DecidablePred Game.turn_fst :=
-  fun turn => by rw [Game.turn_fst] ; exact Nat.decEq (turn % 2) 1
-
-instance : DecidablePred Game.turn_snd :=
-  fun turn => by rw [Game.turn_snd] ; exact Not.decidable
-
-lemma Game.turn_not_fst_iff_snd (turn : ℕ) : (¬ Game.turn_fst turn) ↔ Game.turn_snd turn :=
-  by rw [Game.turn_fst, Game.turn_snd]
-
-lemma Game.turn_not_snd_iff_fst (turn : ℕ) : (¬ Game.turn_snd turn) ↔ Game.turn_fst turn :=
-  by rw [Game.turn_fst, Game.turn_snd, not_ne_iff]
-
-lemma Game.turn_fst_or_snd (turn : ℕ) : Game.turn_fst turn ∨ Game.turn_snd turn :=
-  by rw [Game.turn_fst, Game.turn_snd] ; apply em
 
 
 /-- Computes the history for a given turn, at the end of the turn-/
-def Game.history_on_turn {α β : Type u} (g : Game_World α β)
-    (fst_strat snd_strat: Game.strategy α β) : ℕ → List β
-| 0 => []
-| n+1 => let h := Game.history_on_turn g fst_strat snd_strat n
-         if Game.turn_fst (n+1)
-         then (fst_strat g.init_game_state h) :: h
-         else (snd_strat g.init_game_state h) :: h
+def Game_World.history_on_turn {α β : Type u} (g : Game_World α β)
+    (fst_strat snd_strat: Strategy α β) : ℕ → List β :=
+    History_on_turn g.init_game_state fst_strat snd_strat
+
+lemma Game_World.history_on_turn_def {α β : Type u} (g : Game_World α β) :
+    g.history_on_turn = History_on_turn g.init_game_state :=
+    by
+    rfl
+
+def Symm_Game_World.history_on_turn {α β : Type u} (g : Symm_Game_World α β)
+    (fst_strat snd_strat: Strategy α β) : ℕ → List β :=
+    History_on_turn g.init_game_state fst_strat snd_strat
+
+lemma Symm_Game_World.history_on_turn_def {α β : Type u} (g : Symm_Game_World α β):
+    g.history_on_turn = History_on_turn g.init_game_state :=
+    by
+    rfl
+
+@[simp]
+lemma History_on_turn_World_symm (g : Symm_Game_World α β):
+  g.toGame_World.history_on_turn = g.history_on_turn :=
+  by
+  funext f_st s_st
+  dsimp [Symm_Game_World.history_on_turn, Game_World.history_on_turn, Symm_Game_World.toGame_World]
 
 
 /-- Computes the history for a given turn-/
-def Game.history_on_turn' {α β : Type u} (g : Game α β) : ℕ → List β :=
-  Game.history_on_turn g.toGame_World g.fst_strat g.snd_strat
+def Game.history_on_turn {α β : Type u} (g : Game α β) : ℕ → List β :=
+  History_on_turn g.init_game_state g.fst_strat g.snd_strat
+
+lemma Game.history_on_turn_def {α β : Type u} (g : Game α β) :
+  g.history_on_turn = History_on_turn g.init_game_state g.fst_strat g.snd_strat :=
+  by
+  rfl
+
+def Symm_Game.history_on_turn {α β : Type u} (g : Symm_Game α β) : ℕ → List β :=
+  History_on_turn g.init_game_state g.fst_strat g.snd_strat
 
 
-/-- Computes the state for a given turn, after the action was played-/
-def Game.state_on_turn {α β : Type u} (g : Game_World α β)
-    (fst_strat snd_strat: Game.strategy α β) : ℕ → α
-| 0 => g.init_game_state
-| n+1 => let h := Game.history_on_turn g fst_strat snd_strat n
-         if Game.turn_fst (n+1)
-         then g.fst_transition h (fst_strat g.init_game_state h)
-         else g.snd_transition h (snd_strat g.init_game_state h)
+lemma Symm_Game.history_on_turn_def {α β : Type u} (g : Symm_Game α β) :
+  g.history_on_turn = History_on_turn g.init_game_state g.fst_strat g.snd_strat :=
+  by
+  rfl
+
+@[simp]
+lemma History_on_turn_symm (g : Symm_Game α β):
+  g.toGame.history_on_turn = g.history_on_turn :=
+  by
+  dsimp [Symm_Game.history_on_turn, Game.history_on_turn, Symm_Game.toGame]
+
+@[simp]
+lemma History_on_turn_toWorld (g : Game α β):
+  g.toGame_World.history_on_turn g.fst_strat g.snd_strat = g.history_on_turn :=
+  by
+  dsimp [Game.history_on_turn, Game_World.history_on_turn, Game.toGame_World]
+
+@[simp]
+lemma History_on_turn_symm_toWorld (g : Symm_Game α β):
+  g.toSymm_Game_World.history_on_turn g.fst_strat g.snd_strat = g.history_on_turn :=
+  by
+  dsimp [Symm_Game.history_on_turn, Symm_Game_World.history_on_turn, Symm_Game.toSymm_Game_World]
 
 
-/-- Computes the state for a given turn-/
-def Game.state_on_turn' {α β : Type u} (g : Game α β) : ℕ → α :=
-  Game.state_on_turn g.toGame_World g.fst_strat g.snd_strat
-
-def Game.state_on_turn_neutral {α β : Type u} (g : Game α β) (turn : ℕ) : Prop :=
-  if Game.turn_fst turn
-  then ¬ (g.fst_win_states (g.state_on_turn' turn))
-  else ¬ (g.snd_win_states (g.state_on_turn' turn))
-
--- so one wins by having reach the win state at the end of ones turn
-def Game.fst_win  {α β : Type u} (g : Game α β) : Prop :=
-  ∃ turn : ℕ, Game.turn_fst turn ∧ g.fst_win_states (g.state_on_turn' turn) ∧
-    (∀ t < turn, g.state_on_turn_neutral t)
-
-def Game.snd_win  {α β : Type u} (g : Game α β) : Prop :=
-  ∃ turn : ℕ, Game.turn_snd turn  ∧ g.snd_win_states (g.state_on_turn' turn) ∧
-    (∀ t < turn, g.state_on_turn_neutral t)
 
 
-def Game.is_fst_win  {α β : Type u} (g : Game α β) : Prop :=
-  ∃ ws : Game.strategy α β, ∃ ws_leg : Game.strategy_legal g.init_game_state g.fst_legal ws,
-  ∀ snd_s : Game.strategy α β, (snd_leg : Game.strategy_legal g.init_game_state g.snd_legal snd_s) →
-  {g with  fst_strat := ws, fst_lawful := ws_leg, snd_strat := snd_s, snd_lawful := snd_leg}.fst_win
-
-def Game.is_snd_win  {α β : Type u} (g : Game α β) : Prop :=
-  ∃ ws : Game.strategy α β, ∃ ws_leg : Game.strategy_legal g.init_game_state g.snd_legal ws,
-  ∀ fst_s : Game.strategy α β, (fst_leg : Game.strategy_legal g.init_game_state g.fst_legal fst_s) →
-  {g with  fst_strat := fst_s, fst_lawful := fst_leg, snd_strat := ws, snd_lawful := ws_leg}.snd_win
+-- # Turns
 
 
--- so not including input turn itself, to keep with range convention
-def Game.state_upto_turn {α β : Type u} (g : Game_World α β)
-    (fst_strat snd_strat: Game.strategy α β) (turn : ℕ) : List α :=
-  List.map (Game.state_on_turn g fst_strat snd_strat) (List.range turn)
+
+lemma Turn_not_fst_iff_snd (turn : ℕ) : (¬ Turn_fst turn) ↔ Turn_snd turn :=
+  by rw [Turn_fst, Turn_snd]
+
+lemma Turn_not_snd_iff_fst (turn : ℕ) : (¬ Turn_snd turn) ↔ Turn_fst turn :=
+  by rw [Turn_fst, Turn_snd, not_ne_iff]
+
+lemma Turn_fst_or_snd (turn : ℕ) : Turn_fst turn ∨ Turn_snd turn :=
+  by rw [Turn_fst, Turn_snd] ; apply em
 
 
-def Game.state_upto_turn' {α β : Type u} (g : Game α β) (turn : ℕ) : List α :=
-  List.map g.state_on_turn' (List.range turn)
-
-
-lemma Game.turn_fst_step (turn : ℕ): Game.turn_fst turn ↔ Game.turn_fst (turn + 2) :=
+lemma Turn_fst_step (turn : ℕ): Turn_fst turn ↔ Turn_fst (turn + 2) :=
   by
   constructor
   · intro h
-    rw [Game.turn_fst] at *
+    rw [Turn_fst] at *
     rw [Nat.add_mod]
     rw [h]
     decide
   · intro h
-    rw [Game.turn_fst] at *
+    rw [Turn_fst] at *
     rw [Nat.add_mod] at h
     norm_num at h
     exact h
 
-lemma Game.turn_snd_step (turn : ℕ): Game.turn_snd turn ↔ Game.turn_snd (turn + 2) :=
+lemma Turn_snd_step (turn : ℕ): Turn_snd turn ↔ Turn_snd (turn + 2) :=
   by
-  rw [← Game.turn_not_fst_iff_snd, ← Game.turn_not_fst_iff_snd]
+  rw [← Turn_not_fst_iff_snd, ← Turn_not_fst_iff_snd]
   rw [@not_iff_not]
-  apply Game.turn_fst_step
+  apply Turn_fst_step
 
-lemma Game.turn_fst_snd_step (turn : ℕ): Game.turn_fst turn ↔ Game.turn_snd (turn + 1) :=
+lemma Turn_fst_snd_step (turn : ℕ): Turn_fst turn ↔ Turn_snd (turn + 1) :=
   by
   constructor
   · intro h
-    rw [Game.turn_fst, Game.turn_snd] at *
+    rw [Turn_fst, Turn_snd] at *
     rw [Nat.add_mod]
     rw [h]
     decide
   · intro h
-    rw [Game.turn_fst, Game.turn_snd] at *
+    rw [Turn_fst, Turn_snd] at *
     have := (or_iff_not_imp_right.mp (Nat.mod_two_eq_zero_or_one (turn+1))) h
     rw [Nat.succ_mod_two_eq_zero_iff] at this
     exact this
 
 
-lemma Game.turn_snd_fst_step (turn : ℕ): Game.turn_snd turn ↔ Game.turn_fst (turn + 1) :=
+lemma Turn_snd_fst_step (turn : ℕ): Turn_snd turn ↔ Turn_fst (turn + 1) :=
   by
-  rw [← Game.turn_not_fst_iff_snd, ← @Game.turn_not_snd_iff_fst (turn + 1)]
+  rw [← Turn_not_fst_iff_snd, ← @Turn_not_snd_iff_fst (turn + 1)]
   rw [@not_iff_not]
-  apply Game.turn_fst_snd_step
+  apply Turn_fst_snd_step
+
+
+lemma Turn_fst_not_step (turn : ℕ): Turn_fst turn ↔ ¬ Turn_fst (turn + 1) :=
+  by
+  rw [Turn_not_fst_iff_snd]
+  apply Turn_fst_snd_step
+
+
+lemma Turn_snd_not_step (turn : ℕ): Turn_snd turn ↔ ¬ Turn_snd (turn + 1) :=
+  by
+  rw [Turn_not_snd_iff_fst]
+  apply Turn_snd_fst_step
+
+
+lemma History_on_turn_fst_to_snd (ini : α) (fst_strat snd_strat: Strategy α β) (turn : ℕ):
+  let H := History_on_turn ini fst_strat snd_strat ;
+  Turn_fst turn → H (turn + 1) = (snd_strat ini (H turn)) :: (H turn) :=
+  by
+  intro H tf
+  dsimp [H, History_on_turn]
+  rw [if_neg ((Turn_fst_not_step turn).mp tf)]
+
+lemma History_on_turn_snd_to_fst (ini : α) (fst_strat snd_strat: Strategy α β) (turn : ℕ):
+  let H := History_on_turn ini fst_strat snd_strat ;
+  Turn_snd turn → H (turn + 1) = (fst_strat ini (H turn)) :: (H turn) :=
+  by
+  intro H tf
+  dsimp [H, History_on_turn]
+  rw [if_pos ((Turn_snd_fst_step turn).mp tf)]
+
+lemma Symm_Game_World.history_on_turn_fst_to_snd
+  {α β : Type u} (g : Symm_Game_World α β)
+  (fst_strat snd_strat: Strategy α β) (turn : ℕ):
+  let H := g.history_on_turn fst_strat snd_strat ;
+  Turn_fst turn → H (turn + 1) = (snd_strat g.init_game_state (H turn)) :: (H turn) :=
+  by
+  intro H
+  dsimp [H, Symm_Game_World.history_on_turn]
+  apply History_on_turn_fst_to_snd
+
+lemma Symm_Game_World.history_on_turn_snd_to_fst
+  {α β : Type u} (g : Symm_Game_World α β)
+  (fst_strat snd_strat: Strategy α β) (turn : ℕ):
+  let H := g.history_on_turn fst_strat snd_strat ;
+  Turn_snd turn → H (turn + 1) = (fst_strat g.init_game_state (H turn)) :: (H turn) :=
+  by
+  intro H
+  dsimp [H, Symm_Game_World.history_on_turn]
+  apply History_on_turn_snd_to_fst
+
+
+lemma Game_World.history_on_turn_fst_to_snd
+  {α β : Type u} (g : Game_World α β)
+  (fst_strat snd_strat: Strategy α β) (turn : ℕ):
+  let H := g.history_on_turn fst_strat snd_strat ;
+  Turn_fst turn → H (turn + 1) = (snd_strat g.init_game_state (H turn)) :: (H turn) :=
+  by
+  intro H
+  dsimp [H, Game_World.history_on_turn]
+  apply History_on_turn_fst_to_snd
+
+lemma Game_World.history_on_turn_snd_to_fst
+  {α β : Type u} (g : Game_World α β)
+  (fst_strat snd_strat: Strategy α β) (turn : ℕ):
+  let H := g.history_on_turn fst_strat snd_strat ;
+  Turn_snd turn → H (turn + 1) = (fst_strat g.init_game_state (H turn)) :: (H turn) :=
+  by
+  intro H
+  dsimp [H, Game_World.history_on_turn]
+  apply History_on_turn_snd_to_fst
+
+
+lemma Game.history_on_turn_fst_to_snd
+  {α β : Type u} (g : Game α β) (turn : ℕ):
+  let H := g.history_on_turn ;
+  Turn_fst turn → H (turn + 1) = (g.snd_strat g.init_game_state (H turn)) :: (H turn) :=
+  by
+  intro H
+  dsimp [H, Game.history_on_turn]
+  apply History_on_turn_fst_to_snd
+
+lemma Game.history_on_turn_snd_to_fst
+  {α β : Type u} (g : Game α β) (turn : ℕ):
+  let H := g.history_on_turn ;
+  Turn_snd turn → H (turn + 1) = (g.fst_strat g.init_game_state (H turn)) :: (H turn) :=
+  by
+  intro H
+  dsimp [H, Game.history_on_turn]
+  apply History_on_turn_snd_to_fst
+
+lemma Symm_Game.history_on_turn_fst_to_snd
+  {α β : Type u} (g : Symm_Game α β) (turn : ℕ):
+  let H := g.history_on_turn ;
+  Turn_fst turn → H (turn + 1) = (g.snd_strat g.init_game_state (H turn)) :: (H turn) :=
+  by
+  intro H
+  dsimp [H, Symm_Game.history_on_turn]
+  apply History_on_turn_fst_to_snd
+
+lemma Symm_Game.history_on_turn_snd_to_fst
+  {α β : Type u} (g : Symm_Game α β) (turn : ℕ):
+  let H := g.history_on_turn ;
+  Turn_snd turn → H (turn + 1) = (g.fst_strat g.init_game_state (H turn)) :: (H turn) :=
+  by
+  intro H
+  dsimp [H, Symm_Game.history_on_turn]
+  apply History_on_turn_snd_to_fst
+
+
+
+lemma Invariant_fst {p : ℕ → Prop}
+  (bh : p 1) (ih : ∀ turn : ℕ, Turn_fst turn → p turn → p (turn + 2)):
+  ∀ turn : ℕ, Turn_fst turn → p turn :=
+  by
+  intro t
+  apply @Nat.induct_2_step _ t
+  · intro no
+    rw [Turn_fst] at no
+    contradiction
+  · intro
+    exact bh
+  · intro n a _ c
+    rw [← Turn_fst_step] at c
+    exact ih n c (a c)
+
+
+lemma Invariant_snd {p : ℕ → Prop}
+  (bh : p 0) (ih : ∀ turn : ℕ, Turn_snd turn → p turn → p (turn + 2)):
+  ∀ turn : ℕ, Turn_snd turn → p turn :=
+  by
+  intro t
+  apply @Nat.induct_2_step _ t
+  swap
+  · intro no
+    rw [Turn_snd] at no
+    contradiction
+  · intro
+    exact bh
+  · intro n a _ c
+    rw [← Turn_snd_step] at c
+    exact ih n c (a c)
+
+lemma Invariant_snd' {p : ℕ → Prop}
+  (bh : p 2) (ih : ∀ turn : ℕ, Turn_snd turn → p turn → p (turn + 2)):
+  ∀ turn : ℕ, turn ≥ 2 → Turn_snd turn → p turn :=
+  by
+  intro t
+  apply @Nat.induct_2_step _ t
+  swap
+  · intro no nope
+    rw [Turn_snd] at nope
+    contradiction
+  · intro no
+    linarith
+  · intro n a _ b c
+    rw [← Turn_snd_step] at c
+    cases' n with m
+    · apply bh
+    · cases' m with k
+      · rw [Turn_snd] at c
+        contradiction
+      · apply ih
+        · apply c
+        · apply a _ c
+          rw [Nat.succ_eq_add_one]
+          linarith
+
+
+def Game_World.state_on_turn {α β : Type u} (g : Game_World α β)
+    (fst_strat snd_strat: Strategy α β) : ℕ → α
+| 0 => g.init_game_state
+| n+1 => let h := g.history_on_turn fst_strat snd_strat n
+         if Turn_fst (n+1)
+         then g.fst_transition h (fst_strat g.init_game_state h)
+         else g.snd_transition h (snd_strat g.init_game_state h)
+
+
+/-- Computes the state for a given turn, after the action was played-/
+def Game.state_on_turn {α β : Type u} (g : Game α β) : ℕ → α
+| 0 => g.init_game_state
+| n+1 => let h := g.history_on_turn n
+         if Turn_fst (n+1)
+         then g.fst_transition h (g.fst_strat g.init_game_state h)
+         else g.snd_transition h (g.snd_strat g.init_game_state h)
+
+
+lemma Game.state_on_turn_toWorld {α β : Type u} (g : Game α β):
+  g.toGame_World.state_on_turn g.fst_strat g.snd_strat = g.state_on_turn :=
+  by
+  funext n
+  dsimp [Game.state_on_turn, Game_World.state_on_turn]
+
+
+def Symm_Game_World.state_on_turn {α β : Type u} (g : Symm_Game_World α β)
+    (fst_strat snd_strat: Strategy α β) : ℕ → α
+| 0 => g.init_game_state
+| n+1 => let h := g.history_on_turn fst_strat snd_strat n
+         if Turn_fst (n+1)
+         then g.transition h (fst_strat g.init_game_state h)
+         else g.transition h (snd_strat g.init_game_state h)
+
+
+/-- Computes the state for a given turn, after the action was played-/
+def Symm_Game.state_on_turn {α β : Type u} (g : Symm_Game α β) : ℕ → α
+| 0 => g.init_game_state
+| n+1 => let h := g.history_on_turn n
+         if Turn_fst (n+1)
+         then g.transition h (g.fst_strat g.init_game_state h)
+         else g.transition h (g.snd_strat g.init_game_state h)
+
+
+lemma Symm_Game.state_on_turn_toWorld {α β : Type u} (g : Symm_Game α β):
+  g.toSymm_Game_World.state_on_turn g.fst_strat g.snd_strat = g.state_on_turn :=
+  by
+  funext n
+  dsimp [Symm_Game.state_on_turn, Symm_Game_World.state_on_turn]
+
+@[simp]
+lemma Symm_Game_World.state_on_turn_toGame_World {α β : Type u} (g : Symm_Game_World α β):
+  g.toGame_World.state_on_turn = g.state_on_turn :=
+  by
+  funext f s n
+  --dsimp [Game_World.state_on_turn, Symm_Game_World.state_on_turn]
+  cases n with
+  | zero => dsimp [Game_World.state_on_turn, Symm_Game_World.state_on_turn]
+  | succ m =>
+      dsimp [Game_World.state_on_turn, Symm_Game_World.state_on_turn]
+      congr
+
+@[simp]
+lemma Symm_Game.state_on_turn_toGame {α β : Type u} (g : Symm_Game α β):
+  g.toGame.state_on_turn = g.state_on_turn :=
+  by
+  funext n
+  dsimp [Game.state_on_turn, Symm_Game.state_on_turn]
+
+
+
+-- # State and history by turn
+
+def Game_World.state_on_turn_neutral {α β : Type u} (g : Game_World α β)
+  (f_strat s_strat : Strategy α β) (turn : ℕ) : Prop :=
+  if Turn_fst turn
+  then ¬ (g.fst_win_states (g.state_on_turn f_strat s_strat turn))
+  else ¬ (g.snd_win_states (g.state_on_turn f_strat s_strat turn))
+
+def Symm_Game_World.state_on_turn_neutral {α β : Type u} (g : Symm_Game_World α β)
+  (f_strat s_strat : Strategy α β) (turn : ℕ) : Prop :=
+  if Turn_fst turn
+  then ¬ (g.win_states (g.state_on_turn f_strat s_strat turn))
+  else ¬ (g.win_states (g.state_on_turn f_strat s_strat turn))
+
+
+def Game.state_on_turn_neutral {α β : Type u} (g : Game α β) (turn : ℕ) : Prop :=
+  if Turn_fst turn
+  then ¬ (g.fst_win_states (g.state_on_turn turn))
+  else ¬ (g.snd_win_states (g.state_on_turn turn))
+
+def Symm_Game.state_on_turn_neutral {α β : Type u} (g : Symm_Game α β) (turn : ℕ) : Prop :=
+  if Turn_fst turn
+  then ¬ (g.win_states (g.state_on_turn turn))
+  else ¬ (g.win_states (g.state_on_turn turn))
+
+@[simp]
+lemma Symm_Game.state_on_turn_neutral_toWorld {α β : Type u} (g : Symm_Game α β) :
+  g.toSymm_Game_World.state_on_turn_neutral g.fst_strat g.snd_strat = g.state_on_turn_neutral := by rfl
+
+@[simp]
+lemma Game.state_on_turn_neutral_toWorld {α β : Type u} (g : Game α β) :
+  g.toGame_World.state_on_turn_neutral g.fst_strat g.snd_strat = g.state_on_turn_neutral := by rfl
+
+@[simp]
+lemma Symm_Game.state_on_turn_neutral_toGame {α β : Type u} (g : Symm_Game α β) :
+  g.toGame.state_on_turn_neutral = g.state_on_turn_neutral := by rfl
+
+@[simp]
+lemma Symm_Game_World.state_on_turn_neutral_toWorld {α β : Type u} (g : Symm_Game_World α β):
+  g.toGame_World.state_on_turn_neutral = g.state_on_turn_neutral := by rfl
+
+
+-- so not including input turn itself, to keep with range convention
+def Game_World.state_upto_turn {α β : Type u} (g : Game_World α β)
+    (fst_strat snd_strat: Strategy α β) (turn : ℕ) : List α :=
+  List.map (g.state_on_turn fst_strat snd_strat) (List.range turn)
+
+
+def Game.state_upto_turn {α β : Type u} (g : Game α β) (turn : ℕ) : List α :=
+  List.map g.state_on_turn (List.range turn)
+
+def Symm_Game_World.state_upto_turn {α β : Type u} (g : Symm_Game_World α β)
+    (fst_strat snd_strat: Strategy α β) (turn : ℕ) : List α :=
+  List.map (g.state_on_turn fst_strat snd_strat) (List.range turn)
+
+
+def Symm_Game.state_upto_turn {α β : Type u} (g : Symm_Game α β) (turn : ℕ) : List α :=
+  List.map g.state_on_turn (List.range turn)
+
+
+
+-- # Termination
+
+-- so one wins by having reach the win state at the end of ones turn
+def Game.fst_win  {α β : Type u} (g : Game α β) : Prop :=
+  ∃ turn : ℕ, Turn_fst turn ∧ g.fst_win_states (g.state_on_turn turn) ∧
+    (∀ t < turn, g.state_on_turn_neutral t)
+
+def Game.snd_win  {α β : Type u} (g : Game α β) : Prop :=
+  ∃ turn : ℕ, Turn_snd turn  ∧ g.snd_win_states (g.state_on_turn turn) ∧
+    (∀ t < turn, g.state_on_turn_neutral t)
+
+
+def Game_World.is_fst_win  {α β : Type u} (g : Game_World α β) : Prop :=
+  ∃ ws : Strategy α β,
+  ∀ snd_s : Strategy α β,
+  ∃ ws_leg : Strategy_legal g.init_game_state (fun _ => g.fst_legal) ws snd_s ws,
+   (snd_leg : Strategy_legal g.init_game_state (fun _ => g.snd_legal) ws snd_s snd_s) →
+  ({g with fst_strat := ws, fst_lawful := ws_leg, snd_strat := snd_s, snd_lawful := snd_leg} : Game α β).fst_win
+
+
+def Game_World.is_snd_win  {α β : Type u} (g : Game_World α β) : Prop :=
+  ∃ ws : Strategy α β,
+  ∀ fst_s : Strategy α β,
+  ∃ ws_leg : Strategy_legal g.init_game_state (fun _ => g.snd_legal) fst_s ws ws,
+   (fst_leg : Strategy_legal g.init_game_state (fun _ => g.fst_legal) fst_s ws fst_s) →
+  ({g with fst_strat := fst_s, fst_lawful := fst_leg, snd_strat := ws, snd_lawful := ws_leg} : Game α β).fst_win
+
+
+  -- a draw if all turns are neutral, and one one the players has no legal moves left
+def Game.is_draw {α β : Type u} (g : Game α β) : Prop :=
+  ∃ turn : ℕ, (∀ t ≤ turn, g.state_on_turn_neutral t) ∧
+    ((Turn_fst turn ∧ ∀ act : β, ¬ (g.fst_legal (g.history_on_turn turn) act))
+     ∨
+     (Turn_snd turn ∧ ∀ act : β, ¬ (g.snd_legal (g.history_on_turn turn) act)))
+
+
+-- so one wins by having reach the win state at the end of ones turn
+def Symm_Game.fst_win  {α β : Type u} (g : Symm_Game α β) : Prop :=
+  ∃ turn : ℕ, Turn_fst turn ∧ g.win_states (g.state_on_turn turn) ∧
+    (∀ t < turn, g.state_on_turn_neutral t)
+
+def Symm_Game.snd_win  {α β : Type u} (g : Symm_Game α β) : Prop :=
+  ∃ turn : ℕ, Turn_snd turn  ∧ g.win_states (g.state_on_turn turn) ∧
+    (∀ t < turn, g.state_on_turn_neutral t)
+
+
+def Symm_Game_World.is_fst_win  {α β : Type u} (g : Symm_Game_World α β) : Prop :=
+  ∃ ws : Strategy α β,
+  ∀ snd_s : Strategy α β,
+  ∃ ws_leg : Strategy_legal g.init_game_state (fun _ => g.law) ws snd_s ws,
+   (snd_leg : Strategy_legal g.init_game_state (fun _ => g.law) ws snd_s snd_s) →
+  ({g with fst_strat := ws, fst_lawful := ws_leg, snd_strat := snd_s, snd_lawful := snd_leg} : Symm_Game α β).fst_win
+
+
+def Symm_Game_World.is_snd_win  {α β : Type u} (g : Symm_Game_World α β) : Prop :=
+  ∃ ws : Strategy α β,
+  ∀ fst_s : Strategy α β,
+  ∃ ws_leg : Strategy_legal g.init_game_state (fun _ => g.law) fst_s ws ws,
+   (fst_leg : Strategy_legal g.init_game_state (fun _ => g.law) fst_s ws fst_s) →
+  ({g with fst_strat := fst_s, fst_lawful := fst_leg, snd_strat := ws, snd_lawful := ws_leg} : Symm_Game α β).fst_win
+
+
+  -- a draw if all turns are neutral, and one one the players has no legal moves left
+def Symm_Game.is_draw {α β : Type u} (g : Symm_Game α β) : Prop :=
+  ∃ turn : ℕ, (∀ t ≤ turn, g.state_on_turn_neutral t) ∧
+    ((Turn_fst turn ∧ ∀ act : β, ¬ (g.law (g.history_on_turn turn) act))
+     ∨
+     (Turn_snd turn ∧ ∀ act : β, ¬ (g.law (g.history_on_turn turn) act)))
+
+@[simp]
+lemma Symm_Game.fst_win_toGame  {α β : Type u} (g : Symm_Game α β) :
+  g.toGame.fst_win ↔ g.fst_win := by rfl
+
+@[simp]
+lemma Symm_Game.snd_win_toGame  {α β : Type u} (g : Symm_Game α β) :
+  g.toGame.snd_win ↔ g.snd_win := by rfl
+
+@[simp]
+lemma Symm_Game_World.is_fst_win_toGame  {α β : Type u} (g : Symm_Game_World α β) :
+  g.toGame_World.is_fst_win ↔ g.is_fst_win := by rfl
+
+@[simp]
+lemma Symm_Game_World.snd_win_toGame  {α β : Type u} (g : Symm_Game_World α β) :
+  g.toGame_World.is_snd_win ↔ g.is_snd_win := by rfl
+
+@[simp]
+lemma Symm_Game.is_draw_toGame {α β : Type u} (g : Symm_Game α β) :
+  g.toGame.is_draw ↔ g.is_draw := by rfl
